AwsCryptographicMaterialProviders/dafny/AwsCryptographyKeyStore/src/HierarchicalVersionUtils.dfy
@@ -111,5 +111,60 @@ module {:options "/functionSyntax:4" } HierarchicalVersionUtils {
     (bkcDigest + aes256Key)
   }
 
+  // Helper function to encode encryption context from string map to UTF8 bytes map
+  function EncodeEncryptionContext(
+    input: Structure.EncryptionContextString
+  ): (output: Result<Types.EncryptionContext, string>)
+    ensures output.Success? ==> |output.value| == |input| // Output map size equals input map size
+    ensures output.Failure? ==> output.error == "Unable to encode string"
+  {
+    var encodedEncryptionContext
+      := set k <- input
+           ::
+             (UTF8.Encode(k), UTF8.Encode(input[k]), k);
+
+    if (forall i <- encodedEncryptionContext
+          ::
+            && i.0.Success?
+            && i.1.Success?)
+    then
+      var resultMap := map i <- encodedEncryptionContext :: i.0.value := i.1.value;
+      if |resultMap| == |input| then
+        Success(resultMap)
+      else
+        Failure("Unable to encode string")
+    else
+      Failure("Unable to encode string")
+  }
+
+  // Helper function to decode encryption context from UTF8 bytes map to string map
+  function DecodeEncryptionContext(
+    input: Types.EncryptionContext
+  ): (output: Result<Structure.EncryptionContextString, string>)
+    ensures output.Success? ==> |output.value| == |input| // Output map size equals input map size
+    ensures output.Failure? ==> output.error == "Unable to decode string"
+  {
+    var decodedEncryptionContext
+      := set k <- input
+           ::
+             (UTF8.Decode(k), UTF8.Decode(input[k]), k);
+
+    if (forall i <- decodedEncryptionContext
+          ::
+            && i.0.Success?
+            && i.1.Success?
+               // TODO-UTF8-OPTIMIZATION :: It is silly to Decode and then Encode
+            && var decoded := UTF8.Encode(i.0.value);
+            && decoded.Success?
+            && i.2 == decoded.value)
+    then
+      var resultMap := map i <- decodedEncryptionContext :: i.0.value := i.1.value;
+      if |resultMap| == |input| then
+        Success(resultMap)
+      else
+        Failure("Unable to decode string")
+    else
+      Failure("Unable to decode string")
+  }
 
 }
